WORKS!!!!

src/SDK/Serialize/HeaderV1.dfy
@@ -30,71 +30,249 @@ module HeaderV1 {
   witness *
 
   const VERSION_1: seq<uint8> := [0x01];
+  type Version = s: seq<uint8>
+  | s == VERSION_1
+  witness VERSION_1
+
   const RESERVED_BYTES: seq<uint8> := [0x00, 0x00, 0x00, 0x00];
+  type ReservedBytes = s: seq<uint8>
+  | s == RESERVED_BYTES
+  witness RESERVED_BYTES
 
   function method WriteHeaderBodyV1(
     body: V1HeaderBody
   ):
     (ret: seq<uint8>)
   {
-    var connonicalEC := GetCanonicalEncryptionContext(body.encryptionContext);
+
     var suiteId := GetAlgorithmSuiteId(body.esdkSuiteId);
     var suite := Client.SpecificationClient().GetSuite(suiteId);
 
-    VERSION_1
-    + [body.messageType.Serialize()]
-    + UInt16ToSeq(body.esdkSuiteId)
-    + body.messageId
-    + WriteAADSection(connonicalEC)
+    WriteV1Version(VERSION_1)
+    + WriteV1MessageType(body.messageType)
+    + WriteESDKSuiteId(body.esdkSuiteId)
+    + WriteMessageId(body.messageId)
+    + WriteAADSection(body.encryptionContext)
     + WriteEncryptedDataKeys(body.encryptedDataKeys)
-    + [body.contentType.Serialize()]
-    + RESERVED_BYTES
-    + [suite.encrypt.ivLength]
+    + WriteContentType(body.contentType)
+    + WriteV1ReservedBytes(RESERVED_BYTES)
+    + WriteV1HeaderIvLength(suite.encrypt.ivLength)
     + UInt32ToSeq(body.frameLength)
   }
 
   function method ReadHeaderBodyV1(
-    s: seq<uint8>,
-    pos: nat
-  ):
-    (res: ReadCorrect<V1HeaderBody>)
-    ensures CorrectlyRead(s, pos, res, WriteHeaderBodyV1)
+    bytes: ReadableBytes
+  )
+    :(res: ReadCorrect<V1HeaderBody>)
+    ensures
+      || CorrectlyRead(bytes, res, WriteHeaderBodyV1)
+      // This is to handle the edge case in empty AAD see: `ReadAADSection`
+      || (
+        var headerBytesToAADStart := 20; 
+        var aadStartPosition := bytes.start+headerBytesToAADStart;
+        && res.Success?
+        && aadStartPosition+4 < |bytes.data|
+        && bytes.data[aadStartPosition..aadStartPosition+4] == [0,2,0,0]
+        ==>
+          && CorrectlyRead(bytes, res, WriteExpandedAADSectionHeaderBodyV1))
+
   {
-    var (version, messageTypeStart) :- SerializeFunctions.Read(s, pos, 1);
+    var version :- ReadV1Version(bytes);
 
-    :- Need(version == VERSION_1, Error("Incorrect message version."));
-    var (messageTypeByte, suiteStart) :- Read(s, messageTypeStart, 1);
-    var messageType :- Header.MessageType.Get(messageTypeByte[0]).MapFailure(e => Error(e));
-    var (esdkSuiteId, messageIdStart) :- ReadUInt16(s, suiteStart);
-    :- Need(esdkSuiteId in VALID_IDS, Error("Algorithm suite not supported."));
-    var suiteId := GetAlgorithmSuiteId(esdkSuiteId);
+    var messageType :- ReadV1MessageType(version.tail);
+
+    var esdkSuiteId :- ReadESDKSuiteId(messageType.tail);
+
+    var messageId :- ReadMessageId(esdkSuiteId.tail);
+
+    var encryptionContext :- EncryptionContext2.ReadAADSection(messageId.tail);
+
+    var encryptedDataKeys :- EncryptedDataKeys.ReadEncryptedDataKeysSection(encryptionContext.tail);
+
+    var contentType :- ReadContentType(encryptedDataKeys.tail);
+
+    var reservedBytes :- ReadV1ReservedBytes(contentType.tail);
+
+    var suiteId := GetAlgorithmSuiteId(esdkSuiteId.thing);
     var suite := Client.SpecificationClient().GetSuite(suiteId);
-    var (messageId, ecStart) :- Read(s, messageIdStart, Header.MESSAGE_ID_LEN);
-    var (canonicalEncryptionContext, edkStart) :- EncryptionContext2.ReadAADSection(s, ecStart);
-    var encryptionContext := EncryptionContext2.GetEncryptionContext(canonicalEncryptionContext);
-    LemmaESDKCanonicalEncryptionContextIsESDKEncryptionContext(canonicalEncryptionContext, encryptionContext);
-    var (encryptedDataKeys, contentTypeStart) :- EncryptedDataKeys.ReadEncryptedDataKeysSection(s, edkStart);
-    var (contentTypeByte, reservedStart) :- Read(s, contentTypeStart, 1);
-    var contentType :- Header.ContentType.Get(contentTypeByte[0]).MapFailure(e => Error(e));
-    var (reservedBytes, headerIvLengthStart) :- Read(s, reservedStart, 4);
-    :- Need(RESERVED_BYTES == reservedBytes, Error("Invalid Reserved Bytes"));
-    var (headerIvLengthByte, frameLengthStart) :- Read(s, headerIvLengthStart, 1);
-    var headerIvLength := headerIvLengthByte[0];
-    :- Need(headerIvLength == suite.encrypt.ivLength, Error("Invalid IVLength."));
-    var (frameLength, end) :- ReadUInt32(s, frameLengthStart);
-
-    var body:V1HeaderBody := Header.HeaderBodyV1(
-      messageType := messageType,
-      esdkSuiteId := esdkSuiteId,
-      messageId := messageId,
-      encryptionContext := encryptionContext,
-      encryptedDataKeys := encryptedDataKeys,
-      contentType := contentType,
-      headerIvLength := headerIvLength as nat,
-      frameLength := frameLength
+    var headerIvLength :- ReadV1HeaderIvLength(
+      reservedBytes.tail,
+      suite
     );
 
-    Success((body, end))
+    var frameLength :- ReadUInt32(headerIvLength.tail);
+
+    var body:V1HeaderBody := Header.HeaderBodyV1(
+      messageType := messageType.thing,
+      esdkSuiteId := esdkSuiteId.thing,
+      messageId := messageId.thing,
+      encryptionContext := encryptionContext.thing,
+      encryptedDataKeys := encryptedDataKeys.thing,
+      contentType := contentType.thing,
+      headerIvLength := headerIvLength.thing as nat,
+      frameLength := frameLength.thing
+    );
+
+    Success(Data(body, frameLength.tail))
+  }
+
+  function method WriteV1Version(
+    version: Version
+  ):
+    (ret: seq<uint8>)
+  {
+    version
+  }
+
+  function method ReadV1Version(
+    bytes: ReadableBytes
+  )
+    :(res: ReadCorrect<Version>)
+    ensures CorrectlyRead(bytes, res, WriteV1Version)
+  {
+    var Data(raw, tail) :- SerializeFunctions.Read(bytes, |VERSION_1|);
+    :- Need(raw == VERSION_1, Error("Incorrect message version."));
+    var version: Version := raw;
+    Success(Data(version, tail))
+  }
+
+  function method WriteV1MessageType(
+    messageType: Header.MessageType
+  ):
+    (ret: seq<uint8>)
+  {
+    [messageType.Serialize()]
+  }
+
+  function method ReadV1MessageType(
+    bytes: ReadableBytes
+  )
+    :(res: ReadCorrect<Header.MessageType>)
+    ensures CorrectlyRead(bytes, res, WriteV1MessageType)
+  {
+    var Data(raw, tail) :- SerializeFunctions.Read(bytes, 1);
+    var messageType :- Header.MessageType.Get(raw[0]).MapFailure(e => Error(e));
+    Success(Data(messageType, tail))
+  }
+
+  function method WriteESDKSuiteId(
+    esdkSuiteId: ESDKAlgorithmSuiteId
+  ):
+    (ret: seq<uint8>)
+  {
+    UInt16ToSeq(esdkSuiteId)
+  }
+
+  function method ReadESDKSuiteId(
+    bytes: ReadableBytes
+  )
+    :(res: ReadCorrect<ESDKAlgorithmSuiteId>)
+    ensures CorrectlyRead(bytes, res, WriteESDKSuiteId)
+  {
+    var Data(esdkSuiteId, tail) :- ReadUInt16(bytes);
+    :- Need(esdkSuiteId in VALID_IDS, Error("Algorithm suite ID not supported."));
+    Success(Data(esdkSuiteId, tail))
+  }
+
+  function method WriteMessageId(
+    messageId: Header.MessageID
+  ):
+    (ret: seq<uint8>)
+  {
+    messageId
+  }
+
+  function method ReadMessageId(
+    bytes: ReadableBytes
+  )
+    :(res: ReadBinaryCorrect<Header.MessageID>)
+    ensures CorrectlyRead(bytes, res, WriteMessageId)
+  {
+    SerializeFunctions.Read(bytes, Header.MESSAGE_ID_LEN)
+  }
+
+  function method WriteContentType(
+    contentType: Header.ContentType
+  ):
+    (ret: seq<uint8>)
+  {
+    [contentType.Serialize()]
+  }
+
+  function method ReadContentType(
+    bytes: ReadableBytes
+  )
+    :(res: ReadCorrect<Header.ContentType>)
+    ensures CorrectlyRead(bytes, res, WriteContentType)
+  {
+    var Data(raw, tail) :- SerializeFunctions.Read(bytes, 1);
+    var contentType :- Header.ContentType.Get(raw[0]).MapFailure(e => Error(e));
+    Success(Data(contentType, tail))
+  }
+
+  function method WriteV1ReservedBytes(
+    reservedBytes: ReservedBytes
+  ):
+    (ret: seq<uint8>)
+  {
+    reservedBytes
+  }
+
+  function method ReadV1ReservedBytes(
+    bytes: ReadableBytes
+  )
+    :(res: ReadCorrect<ReservedBytes>)
+    ensures CorrectlyRead(bytes, res, WriteV1ReservedBytes)
+  {
+    var Data(raw, tail) :- SerializeFunctions.Read(bytes, |RESERVED_BYTES|);
+    :- Need(raw == RESERVED_BYTES, Error("Incorrect reserved bytes."));
+    var reservedBytes: ReservedBytes := raw;
+    Success(Data(reservedBytes, tail))
+  }
+
+  function method WriteV1HeaderIvLength(
+    ivLength: uint8
+  ):
+    (ret: seq<uint8>)
+  {
+    [ivLength]
+  }
+
+  function method ReadV1HeaderIvLength(
+    bytes: ReadableBytes,
+    suite: Client.AlgorithmSuites.AlgorithmSuite
+  )
+    :(res: ReadCorrect<uint8>)
+    ensures CorrectlyRead(bytes, res, WriteV1HeaderIvLength)
+  {
+    var Data(raw, tail) :- SerializeFunctions.Read(bytes, 1);
+    :- Need(raw[0] == suite.encrypt.ivLength, Error("HeaderIv Length does not match Algorithm Suite."));
+    Success(Data(raw[0], tail))
+  }
+
+  // This is *not* a function method,
+  // because it is *only* used for correctness.
+  // This represents the sub-optimal encoding of AAD
+  // where empty AAD is encoded with an extra 2 bytes.
+  function WriteExpandedAADSectionHeaderBodyV1(
+    body: V1HeaderBody
+  ):
+    (ret: seq<uint8>)
+  {
+
+    var suiteId := GetAlgorithmSuiteId(body.esdkSuiteId);
+    var suite := Client.SpecificationClient().GetSuite(suiteId);
+
+    WriteV1Version(VERSION_1)
+    + WriteV1MessageType(body.messageType)
+    + WriteESDKSuiteId(body.esdkSuiteId)
+    + WriteMessageId(body.messageId)
+    + WriteExpandedAADSection(body.encryptionContext)
+    + WriteEncryptedDataKeys(body.encryptedDataKeys)
+    + WriteContentType(body.contentType)
+    + WriteV1ReservedBytes(RESERVED_BYTES)
+    + WriteV1HeaderIvLength(suite.encrypt.ivLength)
+    + UInt32ToSeq(body.frameLength)
   }
 
 }
